messageInvariantPrototypes/paxos/decentralizedMonotonic_globalHistory/messageInvariants.dfy
@@ -1,0 +1,442 @@
+include "spec.dfy"
+
+module PaxosMessageInvariants {
+
+import opened Types
+import opened UtilitiesLibrary
+import opened DistributedSystem
+import opened Obligations
+
+// certified self-inductive
+// Every message in the network has a valid source
+ghost predicate ValidMessageSrc(c: Constants, v: Variables) 
+  requires v.WF(c)
+{
+  forall msg | msg in v.network.sentMsgs 
+  :: 
+  match msg 
+    case Prepare(bal) => c.ValidLeaderIdx(bal)
+    case Promise(_, acc, _) => c.ValidAcceptorIdx(acc)
+    case Propose(bal, _) => c.ValidLeaderIdx(bal)
+    case Accept(_, acc) => c.ValidAcceptorIdx(acc)
+}
+
+// Message bundle
+ghost predicate MessageInv(c: Constants, v: Variables) 
+{
+  && v.WF(c)
+  && ValidMessageSrc(c, v)
+  // From Leader transitions
+  // && LeaderValidReceivedPromises(c, v)
+  && ValidProposeMesssage(c, v)
+  // From Acceptor transitions
+  && AcceptorValidAccepted(c, v)
+  && ValidPromiseMessage(c, v)
+  && ValidAcceptMessage(c, v)
+  // // From Learner transitions
+  && LearnerValidReceivedAccepts(c, v)
+  // && ValidLearnMessage(c, v)
+}
+
+lemma InitImpliesMessageInv(c: Constants, v: Variables)
+  requires Init(c, v)
+  ensures MessageInv(c, v)
+{
+}
+
+lemma MessageInvInductive(c: Constants, v: Variables, v': Variables)
+  requires MessageInv(c, v)
+  requires Next(c, v, v')
+  ensures MessageInv(c, v')
+{
+  // InvNextLeaderValidReceivedPromises(c, v, v');
+  InvNextValidProposeMesssage(c, v, v');
+  InvNextAcceptorValidAccepted(c, v, v');
+  InvNextValidPromiseMessage(c, v, v');
+  InvNextValidAcceptMessage(c, v, v');
+  InvNextLearnerValidReceivedAccepts(c, v, v');
+}
+
+/***************************************************************************************
+*                                     Leader Host                                      *
+***************************************************************************************/
+
+// TONY: Whether or not I need the following LeaderValidReceivedPromises invariant
+// affects whether I need to store received messages.
+
+// certified self-inductive
+// Leader updates receivedPromises based on Promise messages
+// Property of Receive
+// ghost predicate LeaderValidReceivedPromises(c: Constants, v: Variables)
+//   requires v.WF(c)
+// {
+//   forall idx, i, p | 
+//     && c.ValidLeaderIdx(idx)
+//     && 0 <= i < |v.leaders[idx].receivedPromises|
+//     && p in v.leaders[idx].receivedPromises[i]
+//   :: 
+//     IsPromiseMessage(v, p)
+// }
+
+// certified self-inductive
+// Property of Send
+ghost predicate ValidProposeMesssage(c: Constants, v: Variables)
+  requires v.WF(c)
+  requires ValidMessageSrc(c, v)
+{
+  forall prop | IsProposeMessage(v, prop)
+  ::
+    (exists i ::
+      && v.ValidHistoryIdx(i)
+      && var ldr := v.History(i).leaders[prop.bal];
+      && ldr.CanPropose(c.leaderConstants[prop.bal])
+      && prop.val == ldr.value
+    )
+}
+
+/***************************************************************************************
+*                                     Acceptor Host                                    *
+***************************************************************************************/
+
+// certified self-inductive
+// Acceptor updates its acceptedVB based on a Propose message carrying that ballot and value
+ghost predicate AcceptorValidAccepted(c: Constants, v: Variables)
+  requires v.WF(c)
+{
+  forall acc, i |
+    && c.ValidAcceptorIdx(acc) 
+    && v.ValidHistoryIdx(i)
+    && v.History(i).acceptors[acc].acceptedVB.Some?
+  :: 
+    && var vb := v.History(i).acceptors[acc].acceptedVB.value;
+    && Propose(vb.b, vb.v) in v.network.sentMsgs
+}
+
+// certified self-inductive
+// Every Promise message ballot reflects acceptor's local promised history, and 
+// it's vbOpt represents a prior accepted value
+// Property of Send
+ghost predicate ValidPromiseMessage(c: Constants, v: Variables) 
+  requires v.WF(c)
+  requires ValidMessageSrc(c, v)
+{
+  forall prom | IsPromiseMessage(v, prom)
+  ::
+  (exists i :: PromiseMessageMatchesHistory(c, v, prom, i))
+}
+
+ghost predicate PromiseMessageMatchesHistory(c: Constants, v: Variables, prom: Message, i: nat)
+  requires v.WF(c)
+  requires ValidMessageSrc(c, v)
+  requires IsPromiseMessage(v, prom)
+{
+  && v.ValidHistoryIdx(i)
+  && v.History(i).acceptors[prom.acc].promised.Some?
+  && prom.bal == v.History(i).acceptors[prom.acc].promised.value
+  && prom.vbOpt == v.History(i).acceptors[prom.acc].acceptedVB
+}
+
+// certified self-inductive
+// Every Accept message reflects acceptor state history
+// Property of Send
+ghost predicate ValidAcceptMessage(c: Constants, v: Variables)
+  requires v.WF(c)
+  requires ValidMessageSrc(c, v)
+{
+  forall accept | IsAcceptMessage(v, accept)
+  ::
+  (exists i :: 
+    && v.ValidHistoryIdx(i)
+    && v.History(i).acceptors[accept.acc].acceptedVB == Some(accept.vb)
+  )
+}
+
+
+/***************************************************************************************
+*                                     Learner Host                                     *
+***************************************************************************************/
+
+// certified self-inductive
+// Learner updates its receivedAccepts map based on a Accept message carrying that 
+// accepted ValBal pair
+// Property of Receive
+ghost predicate LearnerValidReceivedAccepts(c: Constants, v: Variables) 
+  requires v.WF(c)
+{
+  forall idx, vb, acc, i | 
+    && c.ValidLearnerIdx(idx)
+    && v.ValidHistoryIdx(i)
+    && vb in v.History(i).learners[idx].receivedAccepts
+    && acc in v.History(i).learners[idx].receivedAccepts[vb]
+  ::
+    Accept(vb, acc) in v.network.sentMsgs
+}
+
+
+/***************************************************************************************
+*                               Proofs (how unfortunate)                               *
+***************************************************************************************/
+
+
+// lemma InvNextLeaderValidReceivedPromises(c: Constants, v: Variables, v': Variables)
+//   requires v.WF(c)
+//   requires LeaderValidReceivedPromises(c, v)
+//   requires Next(c, v, v')
+//   ensures LeaderValidReceivedPromises(c, v')
+// {
+//   forall idx, i, p | 
+//     && c.ValidLeaderIdx(idx)
+//     && 0 <= i < |v'.leaders[idx].receivedPromises|
+//     && p in v'.leaders[idx].receivedPromises[i]
+//   ensures
+//     IsPromiseMessage(v', p)
+//   {
+//     assert IsPromiseMessage(v, p);  // trigger
+//   }
+// }
+
+
+lemma InvNextValidProposeMesssage(c: Constants, v: Variables, v': Variables)
+  requires v.WF(c)
+  requires ValidMessageSrc(c, v)
+  requires ValidProposeMesssage(c, v)
+  requires Next(c, v, v')
+  ensures ValidProposeMesssage(c, v')
+{
+  forall prop | IsProposeMessage(v', prop)
+  ensures
+    (exists i ::
+      && v'.ValidHistoryIdx(i)
+      && var ldr := v'.History(i).leaders[prop.bal];
+      && ldr.CanPropose(c.leaderConstants[prop.bal])
+      && prop.val == ldr.value
+    )
+  {
+    var dsStep :| NextStep(c, v.Last(), v'.Last(), v.network, v'.network, dsStep);
+    var actor, msgOps := dsStep.actor, dsStep.msgOps;
+    var i: int;
+    if && dsStep.LeaderStep? 
+       && actor == prop.bal
+       && msgOps.send == Some(prop) {
+        // witness
+        i := |v.history| - 1;
+    } else {
+      assert IsProposeMessage(v, prop);
+      // witness
+      i :|       
+          && v.ValidHistoryIdx(i)
+          && var ldr := v.History(i).leaders[prop.bal];
+          && ldr.CanPropose(c.leaderConstants[prop.bal])
+          && prop.val == ldr.value;
+    }
+    // trigger
+      assert  
+        && v'.ValidHistoryIdx(i)
+        && var ldr := v'.History(i).leaders[prop.bal];
+        && ldr.CanPropose(c.leaderConstants[prop.bal])
+        && prop.val == ldr.value;
+  }
+}
+
+lemma InvNextAcceptorValidAccepted(c: Constants, v: Variables, v': Variables)
+  requires v.WF(c)
+  requires AcceptorValidAccepted(c, v)
+  requires Next(c, v, v')
+  ensures AcceptorValidAccepted(c, v')
+{
+  forall acc, i |
+    && c.ValidAcceptorIdx(acc) 
+    && v'.ValidHistoryIdx(i)
+    && v'.History(i).acceptors[acc].acceptedVB.Some?
+  ensures
+    && var vb := v'.History(i).acceptors[acc].acceptedVB.value;
+    && Propose(vb.b, vb.v) in v'.network.sentMsgs
+  {
+    var vb := v'.History(i).acceptors[acc].acceptedVB.value;
+    if Propose(vb.b, vb.v) in v.network.sentMsgs {
+      assert Propose(vb.b, vb.v) in v'.network.sentMsgs;
+    } else {
+      var dsStep :| NextStep(c, v.Last(), v'.Last(), v.network, v'.network, dsStep);
+      if i == |v'.history| - 1 {
+        var actor, msgOps := dsStep.actor, dsStep.msgOps;
+        if && dsStep.AcceptorStep?
+          && actor == acc
+        {
+          assert AcceptorHost.Next(c.acceptorConstants[actor], v.Last().acceptors[actor], v'.Last().acceptors[actor], msgOps);
+          var ac, a, a' := c.acceptorConstants[actor], v.Last().acceptors[actor], v'.Last().acceptors[actor];
+          var step :| AcceptorHost.NextStep(ac, a, a', step, msgOps);
+          if step.MaybeAcceptStep? {
+            assert Propose(vb.b, vb.v) in v'.network.sentMsgs;
+          } else {
+            assert v.History(i-1).acceptors[acc].acceptedVB.Some?;  // trigger
+          }
+        } else {
+          assert v.History(i-1).acceptors[acc].acceptedVB.Some?;  // trigger
+        }
+      } else {
+        assert v.History(i).acceptors[acc].acceptedVB.Some?;  // trigger
+      }
+    }
+  }
+}
+
+lemma InvNextValidPromiseMessage(c: Constants, v: Variables, v': Variables)
+  requires v.WF(c)
+  requires ValidMessageSrc(c, v)
+  requires ValidPromiseMessage(c, v)
+  requires Next(c, v, v')
+  ensures ValidPromiseMessage(c, v')
+{
+  forall prom | IsPromiseMessage(v', prom)
+  ensures
+    exists i :: PromiseMessageMatchesHistory(c, v', prom, i)
+  {
+    var dsStep :| NextStep(c, v.Last(), v'.Last(), v.network, v'.network, dsStep);
+    var actor, msgOps := dsStep.actor, dsStep.msgOps;
+    if && dsStep.AcceptorStep? 
+       && prom.acc == actor 
+       && msgOps.send == Some(prom)
+    {
+      var ac, a, a' := c.acceptorConstants[actor], v.Last().acceptors[actor], v'.Last().acceptors[actor];
+      var step :| AcceptorHost.NextStep(ac, a, a', step, msgOps);
+      if step.MaybePromiseStep? {
+        var doPromise := a.promised.None? || (a.promised.Some? && a.promised.value < a.pendingPrepare.value.bal);
+        if doPromise {
+          assert PromiseMessageMatchesHistory(c, v', prom, |v'.history|-1);  // trigger
+        }
+      }
+    } else {
+      assert IsPromiseMessage(v, prom);  // trigger
+      var i :| PromiseMessageMatchesHistory(c, v, prom, i);  // witness
+      assert PromiseMessageMatchesHistory(c, v', prom, i);   // trigger
+    }
+  }
+}
+
+lemma InvNextValidAcceptMessage(c: Constants, v: Variables, v': Variables)
+  requires v.WF(c)
+  requires ValidMessageSrc(c, v)
+  requires ValidAcceptMessage(c, v)
+  requires Next(c, v, v')
+  ensures ValidAcceptMessage(c, v')
+{
+  forall accept | IsAcceptMessage(v', accept)
+  ensures exists i :: 
+    && v'.ValidHistoryIdx(i)
+    && v'.History(i).acceptors[accept.acc].acceptedVB == Some(accept.vb)
+  {
+    var dsStep :| NextStep(c, v.Last(), v'.Last(), v.network, v'.network, dsStep);
+    var actor, msgOps := dsStep.actor, dsStep.msgOps;
+    if && dsStep.AcceptorStep? 
+       && accept.acc == actor 
+       && msgOps.send == Some(accept)
+    {
+      var ac, a, a' := c.acceptorConstants[actor], v.Last().acceptors[actor], v'.Last().acceptors[actor];
+      var step :| AcceptorHost.NextStep(ac, a, a', step, msgOps);
+      if step.BroadcastAcceptedStep?  {
+        var i := |v'.history|-1;
+        assert  && v'.ValidHistoryIdx(i)  // trigger 
+                && v'.History(i).acceptors[accept.acc].acceptedVB == Some(accept.vb);
+      }
+    } else {
+      var i :|  && v.ValidHistoryIdx(i)   // witness 
+                && v.History(i).acceptors[accept.acc].acceptedVB == Some(accept.vb);
+      assert  && v'.ValidHistoryIdx(i)    // trigger 
+              && v'.History(i).acceptors[accept.acc].acceptedVB == Some(accept.vb);
+    }
+  }
+}
+
+lemma InvNextLearnerValidReceivedAccepts(c: Constants, v: Variables, v': Variables)
+  requires v.WF(c)
+  requires LearnerValidReceivedAccepts(c, v)
+  requires Next(c, v, v')
+  ensures LearnerValidReceivedAccepts(c, v')
+{
+  forall idx, vb, acc, i | 
+    && c.ValidLearnerIdx(idx)
+    && v'.ValidHistoryIdx(i)
+    && vb in v'.History(i).learners[idx].receivedAccepts
+    && acc in v'.History(i).learners[idx].receivedAccepts[vb]
+  ensures
+    && Accept(vb, acc) in v'.network.sentMsgs
+  {
+    if Accept(vb, acc) in v.network.sentMsgs {
+      assert Accept(vb, acc) in v'.network.sentMsgs;
+    } else {
+      var dsStep :| NextStep(c, v.Last(), v'.Last(), v.network, v'.network, dsStep);
+      if i == |v'.history| - 1 {
+        var actor, msgOps := dsStep.actor, dsStep.msgOps;
+        if && dsStep.LearnerStep?
+           && actor == idx
+        {
+          assert LearnerHost.Next(c.learnerConstants[actor], v.Last().learners[actor], v'.Last().learners[actor], msgOps);
+          var lc, l, l' := c.learnerConstants[actor], v.Last().learners[actor], v'.Last().learners[actor];
+          var step :| LearnerHost.NextStep(lc, l, l', step, msgOps);
+          if  && vb in l.receivedAccepts
+              && acc in l.receivedAccepts[vb]
+          {
+            assert  && vb in v.History(i-1).learners[idx].receivedAccepts   // trigger
+                    && acc in v.History(i-1).learners[idx].receivedAccepts[vb];
+          }
+        } else {
+          assert  && vb in v.History(i-1).learners[idx].receivedAccepts     // trigger
+                  && acc in v.History(i-1).learners[idx].receivedAccepts[vb];
+        }
+      } else {
+        assert  && vb in v.History(i).learners[idx].receivedAccepts         // trigger
+                && acc in v.History(i).learners[idx].receivedAccepts[vb];
+      }
+    }
+  }
+}
+
+/***************************************************************************************
+*                                        Utils                                         *
+***************************************************************************************/
+
+ghost predicate IsPrepareMessage(v: Variables, m: Message) {
+  && m.Prepare?
+  && m in v.network.sentMsgs
+}
+
+ghost predicate IsPromiseMessage(v: Variables, m: Message) {
+  && m.Promise?
+  && m in v.network.sentMsgs
+}
+
+ghost predicate IsProposeMessage(v: Variables, m: Message) {
+  && m.Propose?
+  && m in v.network.sentMsgs
+}
+
+ghost predicate IsAcceptMessage(v: Variables, m: Message) {
+  && m.Accept?
+  && m in v.network.sentMsgs
+}
+
+lemma VariableNextProperties(c: Constants, v: Variables, v': Variables, dsStep: Step)
+  requires v.WF(c)
+  requires Next(c, v, v')
+  requires NextStep(c, v.Last(), v'.Last(), v.network, v'.network, dsStep)
+  ensures 1 < |v'.history|
+  ensures v.Last() == v.history[|v'.history|-2] == v'.history[|v'.history|-2]
+  ensures forall i | 0 <= i < |v'.history| - 1 :: v.history[i] == v'.history[i]
+  ensures NextStep(c, v.history[|v'.history|-2], v'.Last(), v.network, v'.network, dsStep)
+{
+  assert 0 < |v.history|;
+  assert 1 < |v'.history|;
+}
+
+lemma GetAcceptorSet(c: Constants, v: Variables)
+returns (accSet: set<AcceptorId>)
+  requires v.WF(c)
+  ensures forall a :: c.ValidAcceptorIdx(a) <==> a in accSet
+  ensures |accSet| == 2 * c.f + 1
+{
+  assert v.history[0].WF(c);  // trigger for |c.acceptorConstants| == 2 * c.f+1
+  accSet := set a |  0 <= a < |c.acceptorConstants|;
+  SetComprehensionSize(|c.acceptorConstants|);
+}
+}  // end module PaxosProof
+
